```haskell

singleton :: a -> [a]
singleton = (:[])

zip :: [a] -> [b] -> [(a, b)]
zip [] _ = []
zip _ [] = []
zip (x:xs) (y:ys) = (x, y) : zip xs ys

foldr :: (a -> b -> b) -> b -> [a] -> b
foldr _ end [] = end
foldr f end (x:xs) =
    let beforeEnd = foldr f end xs
    in f x beforeEnd

foldl :: (b -> a -> b) -> b -> [a] -> b
foldl _ acc [] = acc
foldl f acc (x:xs) =
    let accNext = f x acc
    in foldl f accNext xs

map f xs = foldl (\prev x -> prev ++ [f x]) [] xs

map f xs = foldr (\x rs -> f x : rs) [] xs
map show [1, 2, 3, 4, 5]
    -- f/show, xs/[1, 2, 3, 4, 5], map/foldr..., acc <- []
    = foldr (\x rs -> show x : rs) [] [1, 2, 3, 4, 5]
    -- x <- 1, xs <- [1, 2, 3, 4, 5], foldr/...
    = (\x rs -> show x : rs) 1 (foldr (\x rs -> show x : rs) [] [2, 3, 4, 5])
    -- beta reduction
    = (\rs -> show 1 : rs) (foldr (\x rs -> show x : rs) [] [2, 3, 4, 5])
    -- beta reduction
    = show 1 : foldr (\x rs -> show x : rs) [] [2, 3, 4, 5]
    -- got Weak Head Normal Form!

    -- trying deepseq!
    -- apply show
    = "1" : foldr (\x rs -> show x : rs) [] [2, 3, 4, 5]
    -- apply foldr
    = "1" : show 2 : foldr (\x rs -> show x : rs) [] [3, 4, 5]
    -- apply show
    = "1" : "2" : foldr (\x rs -> show x : rs) [] [3, 4, 5]
    ...
    = "1" : "2" : "3" : "4" : "5" : foldr (\x rs -> show x : rs) [] []
    = "1" : "2" : "3" : "4" : "5" : []

```
